reverted to more powerful sup in lattice.v, tower helpers in rel.v

theories/rel.v
@@ -1,29 +1,14 @@
 (** * Utilities for working with binary relations  *)
 
-Require Import coinduction.
+Require Import tower.
 Set Implicit Arguments.
 
 (* TODO: 
-   - fix slowness
-   - contextual functions for relations of arbitrary arity?
-   - contexts of arbitrary arity?
    - sharing with relation algebra
  *)
   
 
 (** * Generic definitions and results about relations *)
-
-(** pairs and sets of pairs *)
-
-Definition pair A (x y: A) := fun x' y' => x=x' /\ y=y'.
-Lemma leq_pair A (x y: A) (R: A -> A -> Prop): R x y <-> pair x y <= R.
-Proof. firstorder congruence. Qed.
-Global Opaque pair.
-
-(** squaring function *)
-Program Definition square {A}: mon (A -> A -> Prop) :=
-  {| body R x y := exists2 z, R x z & R z y |}.
-Next Obligation. cbv. firstorder. Qed. 
 
 (** converse function (an involution) *)
 Program Definition converse {A}: mon (A -> A -> Prop) :=
@@ -33,318 +18,126 @@ Next Obligation. cbv. firstorder. Qed.
 #[export] Instance Involution_converse {A}: Involution (@converse A).
 Proof. now intros ? ?. Qed.
 
-Section s.
-  Variables (A: Type) (b: mon (relation A)).
-  Notation t := (t b).
-  Notation T := (T b).
-  Notation bt := (bt b).
-  Notation bT := (bT b).
-
-  (* TOTHINK: we need to expand [eq] below in order to avoid universe inconsistencies with [RelationAlgebra.srel]; not so clear why... *)
-  Notation const_eq := (const (fun x y => x=y)).
-
-  (** [gfp] is always a subrelation of [t R], [bt R], [T f R], and [bT f R] 
-      TOTHINK: declare other links in the lattice?
-      (bt<=bT<=T and bt<=t<=T)
-   *)
-  Global Instance subrelation_gfp_T f (R: relation A): subrelation (gfp b) (T f R).
-  Proof. refine (gfp_T _ _ R). Qed.
-  
-  Global Instance subrelation_gfp_t (R: relation A): subrelation (gfp b) (t R).
-  Proof. refine (gfp_t _ R). Qed.
-
-  (** the next two are not declared as instances by default, 
-      in order to circumvent setoid_rewriting inefficiencies *)
-  Lemma subrelation_gfp_bt (R: relation A): subrelation (gfp b) (bt R).
-  Proof. refine (gfp_bt _ R). Qed.
-  
-  Lemma subrelation_gfp_bT f (R: relation A): subrelation (gfp b) (bT f R).
-  Proof. refine (gfp_bT _ _ R). Qed.
-
-  (** helpers to prove that relations are reflexive/symmetric/transitive from algebraic properties *)
-  Lemma build_reflexive (R: relation A): const_eq R <= R -> Reflexive R.
-  Proof. intros H x. now apply H. Qed.
-  Lemma build_symmetric (R: relation A): converse R <= R -> Symmetric R.
-  Proof. intros H x y xy. now apply H. Qed.
-  Lemma build_transitive (R: relation A): square R <= R -> Transitive R.
-  Proof. intros H x y z xy yz. now apply H; exists y. Qed.
-  Lemma build_preorder (R: relation A): const_eq R <= R -> square R <= R -> PreOrder R.
-  Proof.
-    split.
-    now apply build_reflexive.
-    now apply build_transitive.
-  Qed.
-  Lemma build_equivalence (R: relation A): const_eq R <= R -> converse R <= R -> square R <= R -> Equivalence R.
-  Proof.
-    split.
-    now apply build_reflexive.
-    now apply build_symmetric.
-    now apply build_transitive.
-  Qed.
-  
-  (** provided that [const eq], [square], and [converse] are below [t], 
-    we have that [gfp b], [t R], [bt R], [T f R], and [bT f R] are always equivalence relations. *)
-  (* TOTHINK: use the transfer lemmas [Pt_PT, Pt_Pbt, Pt_PbT]? *)
-  (* TOTHINK: setup typclasses to avoid repetitions? *)
-  Hypothesis eq_t: const_eq <= t.
-  Hypothesis square_t: square <= t.
-  Lemma PreOrder_t R: PreOrder (t R).
-  Proof. apply build_preorder; now apply ft_t. Qed.
-  Corollary PreOrder_gfp: PreOrder (gfp b).
-  Proof. apply PreOrder_t. Qed.
-  Lemma PreOrder_T f R: PreOrder (T f R).
-  Proof. apply build_preorder; now apply fT_T. Qed.   (* TOFIX: slow Qed *)
-  Lemma PreOrder_bt R: PreOrder (bt R).
-  Proof. apply build_preorder; now apply fbt_bt. Qed.
-  Lemma PreOrder_bT f R: PreOrder (bT f R).
-  Proof. apply build_preorder; now apply fbT_bT. Qed.
-
-  Hypothesis converse_t: converse <= t.
-  Lemma Equivalence_t R: Equivalence (t R).
-  Proof. apply build_equivalence; now apply ft_t. Qed.
-  Corollary Equivalence_gfp: Equivalence (gfp b).
-  Proof. apply Equivalence_t. Qed.
-  Lemma Equivalence_T f R: Equivalence (T f R).
-  Proof. apply build_equivalence; now apply fT_T. Qed. (* TOFIX: slow Qed *)
-  Lemma Equivalence_bt R: Equivalence (bt R).
-  Proof. apply build_equivalence; now apply fbt_bt. Qed. (* TOFIX: slow proof *)
-  Lemma Equivalence_bT f R: Equivalence (bT f R).
-  Proof. apply build_equivalence; now apply fbT_bT. Qed. (* TOFIX: slow proof *)
-End s.
-
-
-(** * Contexts closure functions *)
-
-Section context.
-Variable S: Type.
-Section unary. 
-Variable f: S -> S. 
-
-(** unary context: [unary_ctx f](R) = {(f x, f y) | x R y }  *)
-Program Definition unary_ctx: mon (S -> S -> Prop) :=
-  {| body R := sup_all (fun x =>
-               sup (R x) (fun x' => pair (f x) (f x'))) |}.
-Next Obligation.
-  Transparent pair. Opaque plus.
-  cbv; firstorder subst; eauto.
-  Transparent plus. Opaque pair.
-Qed.
-
-Lemma leq_unary_ctx R T:
-  unary_ctx R <= T <-> forall x x', R x x' -> T (f x) (f x').
-Proof.
-  unfold unary_ctx. setoid_rewrite sup_all_spec.
-  setoid_rewrite sup_spec.
-  setoid_rewrite <-leq_pair. firstorder. 
-Qed.
-Lemma in_unary_ctx (R: S -> S -> Prop) x x':
-  R x x' -> unary_ctx R (f x) (f x').
-Proof. intros. now apply ->leq_unary_ctx. Qed.
-Global Opaque unary_ctx.
-
-(** context functions are always symmetric *)
-Lemma unary_sym: compat converse unary_ctx.
-Proof. intro R. simpl. apply leq_unary_ctx. intros. now apply in_unary_ctx. Qed.
-
-(** helper lemmas to prove that a unary context function is below the companion *)
-Lemma unary_ctx_b b c:
-  unary_ctx ° b <= c <-> forall R, Proper (b R ==> c R) f.
-Proof.
-  split; intro H.
-  - intros R p q pq. apply H. now apply in_unary_ctx.
-  - intro R. apply leq_unary_ctx. apply H.
-Qed.
-Corollary unary_ctx_t (b: mon (S -> S -> Prop)):
-  (forall R, Proper (b R ==> bT b unary_ctx R) f) ->
-  unary_ctx <= t b.
-Proof. intro H. apply Coinduction. now apply unary_ctx_b. Qed.
-Corollary unary_ctx_t_sym_ (b s: mon (S -> S -> Prop)) {H: Sym_from converse b s}:
-  (forall R, Proper (b R ==> s (T b unary_ctx R)) f) ->
-  unary_ctx <= t b.
-Proof.
-  intro. apply Coinduction, by_Symmetry. apply unary_sym.
-  apply <- unary_ctx_b.
-  exact H0.                     (* TOFIX: slow *)
-Qed.                            (* TOFIX: slow too *)
-
-
-(** if it is below [t], then the function [f] always preserves [t R], [bt R], [T f R], [bT f R] *)
-Lemma unary_proper_t b:
-  unary_ctx <= t b -> forall R, Proper (t b R ==> t b R) f.
-Proof. intros H R x x' Hx. apply (ft_t H). now apply in_unary_ctx. Qed.
-Lemma unary_proper_bt b:
-  unary_ctx <= t b -> forall R, Proper (bt b R ==> bt b R) f.
-Proof. intros H R x x' Hx. apply (fbt_bt H). now apply in_unary_ctx. Qed.
-Lemma unary_proper_T b g:
-  unary_ctx <= t b -> forall R, Proper (T b g R ==> T b g R) f.
-Proof. intros H R x x' Hx. apply (fT_T H). now apply in_unary_ctx. Qed. (* TOFIX: slow *)
-Lemma unary_proper_bT b g:
-  unary_ctx <= t b -> forall R, Proper (bT b g R ==> bT b g R) f.
-Proof. intros H R x x' Hx. apply (fbT_bT H). now apply in_unary_ctx. Qed.
-
-Global Instance unary_proper_Tctx b R:
-  Proper (T b unary_ctx R ==> T b unary_ctx R) f.
-Proof. intros x x' Hx. apply (fTf_Tf b). now apply in_unary_ctx. Qed. (* TOFIX: slow Qed *)
-
-End unary.
-Section binary. 
-Variable f: S -> S -> S. 
-                                 
-(** binary context: [unary_ctx f](R) = {(f x x', f y y') | x R y, x' R y' }  *)
-Program Definition binary_ctx: mon (S -> S -> Prop) :=
-  {| body R := sup_all (fun x =>
-               sup_all (fun y => 
-               sup (R x) (fun x' => 
-               sup (R y) (fun y' => pair (f x y) (f x' y'))))) |}.
-Next Obligation.
-  Transparent pair. Opaque plus.
-  cbv; firstorder subst; eauto 8.
-  Transparent plus. Opaque pair.
-Qed.
-
-Lemma leq_binary_ctx R T:
-  binary_ctx R <= T <-> forall x x', R x x' -> forall y y', R y y' -> T (f x y) (f x' y').
-Proof.
-  unfold binary_ctx. do 2 setoid_rewrite sup_all_spec.
-  do 2 setoid_rewrite sup_spec.
-  setoid_rewrite <-leq_pair. firstorder. 
-Qed.
-Lemma in_binary_ctx (R: S -> S -> Prop) x x' y y':
-  R x x' -> R y y' -> binary_ctx R (f x y) (f x' y').
-Proof. intros. now apply ->leq_binary_ctx. Qed.
-Global Opaque binary_ctx.
-
-(** such a function is always symmetric *)
-Lemma binary_sym: compat converse binary_ctx.
-Proof. intro R. simpl. apply leq_binary_ctx. intros. now apply in_binary_ctx. Qed.
-
-(** helper lemmas to prove that a binary context function is below the companion *)
-Lemma binary_ctx_b b c:
-  binary_ctx ° b <= c  <-> forall R, Proper (b R ==> b R ==> c R) f.
-Proof.
-  split; intro H.
-  - intros R p q pq u v uv. apply H. now apply in_binary_ctx.
-  - intro R. apply leq_binary_ctx. apply H.
-Qed.
-Corollary binary_ctx_t (b: mon (S -> S -> Prop)):
-  (forall R, Proper (b R ==> b R ==> bT b binary_ctx R) f) ->
-  binary_ctx <= t b.
-Proof. intro H. apply Coinduction. now apply binary_ctx_b. Qed.
-Corollary binary_ctx_t_sym_ (b s: mon (S -> S -> Prop)) {H: Sym_from converse b s}:
-  (forall R, Proper (b R ==> b R ==> s (T b binary_ctx R)) f) ->
-  binary_ctx <= t b.
-Proof. intro. apply Coinduction, by_Symmetry. apply binary_sym. now apply binary_ctx_b. Qed. (* TOFIX: slow *)
-
-(** if it is below [t], then the function [f] always preserves [t R], [bt R], [T f R], [bT f R] *)
-Lemma binary_proper_t b:
-  binary_ctx <= t b -> forall R, Proper (t b R ==> t b R ==> t b R) f.
-Proof. intros H R x x' Hx y y' Hy. apply (ft_t H). now apply in_binary_ctx. Qed.
-Lemma binary_proper_bt b:
-  binary_ctx <= t b -> forall R, Proper (bt b R ==> bt b R ==> bt b R) f.
-Proof. intros H R x x' Hx y y' Hy. apply (fbt_bt H). now apply in_binary_ctx. Qed.
-Lemma binary_proper_T b g:
-  binary_ctx <= t b -> forall R, Proper (T b g R ==> T b g R ==> T b g R) f.
-Proof. intros H R x x' Hx y y' Hy. apply (fT_T H). now apply in_binary_ctx. Qed. (* TOFIX: slow Qed *)
-Lemma binary_proper_bT b g:
-  binary_ctx <= t b -> forall R, Proper (bT b g R ==> bT b g R ==> bT b g R) f.
-Proof. intros H R x x' Hx y y' Hy. apply (fbT_bT H). now apply in_binary_ctx. Qed.
-
-Global Instance binary_proper_Tctx b R:
-  Proper (T b binary_ctx R ==> T b binary_ctx R ==> T b binary_ctx R) f.
-Proof. intros x x' Hx y y' Hy. apply (fTf_Tf b). now apply in_binary_ctx. Qed. (* TOFIX: slow Qed *)
-
-End binary.
-Section ternary. 
-Variable f: S -> S -> S -> S. 
-
-                                 
-(** ternary context: [ternary_ctx f](R) = {(f x x' x'', f y y' y'') | x R y, x' R y', x'' R y'' }  *)
-Program Definition ternary_ctx: mon (S -> S -> Prop) :=
-  {| body R := sup_all (fun x =>
-               sup_all (fun y => 
-               sup_all (fun z => 
-               sup (R x) (fun x' => 
-               sup (R y) (fun y' => 
-               sup (R z) (fun z' => pair (f x y z) (f x' y' z'))))))) |}.
-Next Obligation.
-  Transparent pair. Opaque plus.
-  cbv; firstorder subst; eauto 8.
-  Transparent plus. Opaque pair.
-Qed.
-
-Lemma leq_ternary_ctx R T:
-  ternary_ctx R <= T <->
-  forall x x', R x x' -> forall y y', R y y' -> forall z z', R z z' -> T (f x y z) (f x' y' z').
-Proof.
-  unfold ternary_ctx. do 3 setoid_rewrite sup_all_spec.
-  do 3 setoid_rewrite sup_spec.
-  setoid_rewrite <-leq_pair. firstorder. 
-Qed.
-Lemma in_ternary_ctx (R: S -> S -> Prop) x x' y y' z z':
-  R x x' -> R y y' -> R z z' -> ternary_ctx R (f x y z) (f x' y' z').
-Proof. intros. now apply ->leq_ternary_ctx. Qed.
-Global Opaque ternary_ctx.
-
-(** such a function is always symmetric *)
-Lemma ternary_sym: compat converse ternary_ctx.
-Proof. intro R. simpl. apply leq_ternary_ctx. intros. now apply in_ternary_ctx. Qed.
-
-(** helper lemmas to prove that a ternary context function is below the companion *)
-Lemma ternary_ctx_b b c:
-  ternary_ctx ° b <= c <-> forall R, Proper (b R ==> b R ==> b R ==> c R) f.
-Proof.
-  split; intro H.
-  - intros R p q pq u v uv s t st. apply H. now apply in_ternary_ctx.
-  - intro R. apply leq_ternary_ctx. apply H.
-Qed.
-Corollary ternary_ctx_t (b: mon (S -> S -> Prop)):
-  (forall R, Proper (b R ==> b R ==> b R ==> bT b ternary_ctx R) f) ->
-  ternary_ctx <= t b.
-Proof. intro H. apply Coinduction. now apply ternary_ctx_b. Qed.
-Corollary ternary_ctx_t_sym_ (b s: mon (S -> S -> Prop)) {H: Sym_from converse b s}:
-  (forall R, Proper (b R ==> b R ==> b R ==> s (T b ternary_ctx R)) f) ->
-  ternary_ctx <= t b.
-Proof. intro. apply Coinduction, by_Symmetry. apply ternary_sym. now apply ternary_ctx_b. Qed. (* TOFIX: slow *)
-
-(** if it is below [t], then the function [f] always preserves [t R], [bt R], [T f R], [bT f R] *)
-Lemma ternary_proper_t b:
-  ternary_ctx <= t b -> forall R, Proper (t b R ==> t b R ==> t b R ==> t b R) f.
-Proof. intros H R x x' Hx y y' Hy z z' Hz. apply (ft_t H). now apply in_ternary_ctx. Qed.
-Lemma ternary_proper_bt b:
-  ternary_ctx <= t b -> forall R, Proper (bt b R ==> bt b R ==> bt b R ==> bt b R) f.
-Proof. intros H R x x' Hx y y' Hy z z' Hz. apply (fbt_bt H). now apply in_ternary_ctx. Qed.
-Lemma ternary_proper_T b g:
-  ternary_ctx <= t b -> forall R, Proper (T b g R ==> T b g R ==> T b g R ==> T b g R) f.
-Proof. intros H R x x' Hx y y' Hy z z' Hz. apply (fT_T H). now apply in_ternary_ctx. Qed. (* TOFIX: slow Qed *)
-Lemma ternary_proper_bT b g:
-  ternary_ctx <= t b -> forall R, Proper (bT b g R ==> bT b g R ==> bT b g R ==> bT b g R) f.
-Proof. intros H R x x' Hx y y' Hy z z' Hz. apply (fbT_bT H). now apply in_ternary_ctx. Qed.
-
-Global Instance ternary_proper_Tctx b R:
-  Proper (T b ternary_ctx R ==> T b ternary_ctx R ==> T b ternary_ctx R ==> T b ternary_ctx R) f.
-Proof. intros x x' Hx y y' Hy z z' Hz. apply (fTf_Tf b). now apply in_ternary_ctx. Qed. (* TOFIX: slow Qed *)
-
-End ternary.
-End context.
-
-(** reexporting those three lemmas with different argument order to help typeclasss resolution *)
-Definition unary_ctx_t_sym {S b s H} f := @unary_ctx_t_sym_ S f b s H. 
-Definition binary_ctx_t_sym {S b s H} f := @binary_ctx_t_sym_ S f b s H. 
-Definition ternary_ctx_t_sym {S b s H} f := @ternary_ctx_t_sym_ S f b s H. 
-
-Transparent pair.
-Lemma converse_pair A (p q: A): converse (pair p q) == pair q p.
-Proof. unfold pair, converse; split; simpl; tauto. Qed.
-Global Opaque pair.
-
-Lemma converse_sup S I P (f: I -> relation S):
-  converse (sup P f) == sup P (fun i => converse (f i)).
-Proof. simpl. firstorder. Qed.
+(* TODO: used? generalise? *)
+Lemma converse_sup {A} (P: (A -> A -> Prop) -> Prop): converse (sup P) == sup' P converse. 
+Proof. apply invol_sup. Qed.
 
 Lemma converse_cup S (R R': relation S):
   converse (cup R R') == cup (converse R) (converse R').
-Proof. simpl. firstorder. Qed.
+Proof. apply invol_cup. Qed.
 
-Lemma converse_square S (R: relation S):
-  converse (square R) == square (converse R).
-Proof. simpl. firstorder. Qed.
+Lemma converse_cap S (R R': relation S):
+  converse (cap R R') == cap (converse R) (converse R').
+Proof. apply invol_cap. Qed.
+
+
+Section s.
+  Context {A: Type}.
+          
+  (** helpers for proving reflexivity/symmetry/transitivity of chain elements *)
+  Lemma inf_closed_reflexive: inf_closed (@Reflexive A).
+  Proof. cbv. firstorder. Qed.
+  Lemma inf_closed_symmetric: inf_closed (@Symmetric A).
+  Proof. cbv. firstorder. Qed.
+  Lemma inf_closed_transitive: inf_closed (@Transitive A).
+  Proof. cbv; firstorder eauto. Qed.
+
+  Context {b: mon (relation A)}.
+
+  (** for chain elements [R], [gfp b] and [b R] are always subrelations of [R] *)
+  #[export] Instance sub_bChain {R} {CR: Chain b R}: subrelation (b R) R.
+  Proof. exact (b_chain (b:=b)). Qed.
+  #[export] Instance sub_gfp_Chain {R} {CR: Chain b R}: subrelation (gfp b) R.
+  Proof. exact (gfp_chain (b:=b)). Qed.
+  
+  Proposition Reflexive_chain: (forall R, Chain b R -> Reflexive R -> Reflexive (b R)) -> forall R, Chain b R -> Reflexive R.
+  Proof. apply tower, inf_closed_reflexive. Qed.  
+  Proposition Symmetric_chain: (forall R, Chain b R -> Symmetric R -> Symmetric (b R)) -> forall R, Chain b R -> Symmetric R.
+  Proof. apply tower, inf_closed_symmetric. Qed.  
+  Proposition Transitive_chain: (forall R, Chain b R -> Transitive R -> Transitive (b R)) -> forall R, Chain b R -> Transitive R.
+  Proof. apply tower, inf_closed_transitive. Qed.
+
+  (** helpers for proving that n-ary functions preserve chain elements *)
+  Fixpoint nfun n :=
+    match n with
+    | 0 => A
+    | S n => A -> nfun n
+    end.
+  Fixpoint respectful_iter n R S: relation (nfun n) :=
+    match n with
+    | 0 => S
+    | S n => respectful R (respectful_iter n R S)
+    end.
+  Lemma inf_closed_respectful n f g: inf_closed (fun R => respectful_iter n R R f g).
+  Proof.
+    induction n; intros P HP.
+    - apply HP.
+    - intros x y xy. apply IHn. 
+      intros R HR. apply HP. apply HR. apply xy, HR.
+  Qed.
+  Corollary inf_closed_proper n f: inf_closed (fun R => Proper (respectful_iter n R R) f).
+  Proof. apply inf_closed_respectful. Qed.
+
+  Proposition Proper_chain n f:
+    (forall R, Chain b R -> Proper (respectful_iter n R R) f -> Proper (respectful_iter n (b R) (b R)) f) ->
+    forall R, Chain b R -> Proper (respectful_iter n R R) f.
+  Proof. exact (tower (inf_closed_proper n f)). Qed.
+
+  (** symmetry arguments *)
+
+  Section sym.
+    
+   Context {s} {I: Symmetrical converse b s}.
+
+   Section s.
+    Context {R} {CR: Chain b R}.
+  
+    Lemma Sym_converse: converse R == R.
+    Proof. apply invol_chain. Qed.
+  
+    Lemma Sym_biff x y: b R x y <-> s R x y /\ s R y x.
+    Proof. exact (symmetrical_chain (x:=R) x y). Qed.
+  
+    Lemma Sym_Reflexive_chain: Reflexive (s R) -> Reflexive (b R).
+    Proof. intros H x. now apply Sym_biff; split. Qed.
+  
+    Lemma Sym_Transitive_chain: Transitive (s R) -> Transitive (b R).
+    Proof. intros H x y z. rewrite 3Sym_biff. intuition; etransitivity; eauto. Qed.
+  
+    Lemma Sym_respectful_chain n f g:
+      respectful_iter n (b R) (s R) f g ->
+      respectful_iter n (b R) (s R) g f ->
+      respectful_iter n (b R) (b R) f g.
+    Proof.
+      induction n; cbn; intros H H'.
+      - now apply Sym_biff. 
+      - intros x y xy. apply IHn. apply H, xy.
+        apply H'. revert xy. rewrite 2Sym_biff. tauto.
+    Qed.
+    
+    Corollary Sym_Proper_chain n f: Proper (respectful_iter n (b R) (s R)) f -> Proper (respectful_iter n (b R) (b R)) f.
+    Proof. intro. now apply Sym_respectful_chain. Qed.
+
+   End s.
+   
+   Proposition Reflexive_symchain:
+     (forall R, Chain b R -> Reflexive R -> Reflexive (s R)) ->
+     forall R, Chain b R -> Reflexive R.
+   Proof. intro. apply Reflexive_chain. intros. apply Sym_Reflexive_chain; auto. Qed.  
+    
+   Proposition Symmetric_symchain:
+     (** this one is granted *)
+     forall R, Chain b R -> Symmetric R.
+   Proof. intros. change (R <= converse R). now rewrite Sym_converse. Qed.
+
+   Proposition Transitive_symchain:
+     (forall R, Chain b R -> Transitive R -> Transitive (s R)) ->
+     forall R, Chain b R -> Transitive R.
+   Proof. intro. apply Transitive_chain. intros. apply Sym_Transitive_chain; auto. Qed.
+
+   Proposition Proper_symchain n f:
+     (forall R, Chain b R -> Proper (respectful_iter n R R) f -> Proper (respectful_iter n (b R) (s R)) f) ->
+     forall R, Chain b R -> Proper (respectful_iter n R R) f.
+   Proof. intro. apply Proper_chain. intros. apply Sym_Proper_chain; auto. Qed.
+  End sym. 
+End s.
